Prove an end-to-end result for the femtokernel. Some bureaucratic proofs still missing.

case_study/RiscvPmp/FemtoKernel.v
@@ -34,6 +34,7 @@ From Katamaran Require Import
      Bitvector
      Notations
      Specification
+     SmallStep.Step
      RiscvPmp.BlockVer.Spec
      RiscvPmp.BlockVer.Verifier
      RiscvPmp.IrisModel
@@ -46,7 +47,7 @@ From Katamaran Require
      RiscvPmp.Model.
 From iris.base_logic Require lib.gen_heap lib.iprop invariants.
 From iris.bi Require interface big_op.
-From iris.algebra Require dfrac.
+From iris.algebra Require dfrac big_op.
 From iris.program_logic Require weakestpre adequacy.
 From iris.proofmode Require string_ident tactics.
 From stdpp Require namespaces.
@@ -710,3 +711,171 @@ Import BlockVerificationDerived2.
       }
       now iApply LoopVerification.valid_semTriple_loop.
   Qed.
+
+  Definition mem_has_instr (μ : Memory) (a : Z) (instr : AST) : Prop :=
+    exists v, μ a = v /\ pure_decode v = inr instr.
+
+  Fixpoint mem_has_instrs (μ : Memory) (a : Z) (instrs : list AST) : Prop :=
+    match instrs with
+    | cons inst instrs => mem_has_instr μ a inst /\ mem_has_instrs μ (4 + a) instrs
+    | nil => True
+    end.
+
+  Import RiscvPmpSemantics.
+  Import SmallStepNotations.
+
+  Import iris.bi.big_op.
+  Import iris.algebra.big_op.
+
+  Lemma liveAddrs_split : liveAddrs = seqZ 0 72 ++ seqZ 72 12 ++ [84 : Z] ++ seqZ 85 3 ++ advAddrs.
+  Proof.
+    (* TODO: scalable proof *)
+    by compute.
+  Qed.
+
+  Lemma intro_ptsto_instrs `{sailGS Σ} {μ : Memory} {a : Z} {instrs : list AST} :
+    mem_has_instrs μ a instrs ->
+    ([∗ map] k ↦ y ∈ list_to_map (map (λ a : Z, (a, μ a)) (seqZ a (4 * length instrs))), interp_ptsto k y)
+      ⊢ ptsto_instrs a instrs.
+  Proof.
+    iIntros (Hmeminstrs) "Hmem".
+    iInduction instrs as [|instr instrs] "IH" forall (a Hmeminstrs).
+    - done.
+    - do 4 (rewrite seqZ_cons; last (by cbn)).
+      cbn in *.
+      destruct Hmeminstrs as [(v & <- & Hv) Hmeminstrs].
+      rewrite ?big_sepM_insert.
+      + iDestruct "Hmem" as "(Hmema & _ & _ & _ & Hmem)".
+        iSplitL "Hmema".
+        * unfold interp_ptsto_instr.
+          iExists (μ a).
+          now iFrame.
+        * replace (a + 4)%Z with (4 + a)%Z by lia.
+          iApply "IH".
+          {now iPureIntro.}
+          replace (Z.pred (Z.pred (Z.pred (Z.pred (4 * S (length instrs)))))) with (4 * length instrs)%Z by lia.
+          replace (Z.succ (Z.succ (Z.succ (Z.succ a)))) with (4 + a)%Z by lia.
+          iExact "Hmem".
+      + admit.
+      + admit.
+      + admit.
+      + admit.
+  Admitted.
+
+  Lemma intro_ptstoSthL `{sailGS Σ} (μ : Memory) (addrs : list Z)  :
+    NoDup addrs ->
+    ([∗ map] k↦y ∈ (list_to_map (map (λ a : Z, (a, μ a)) addrs)), gen_heap.mapsto k (dfrac.DfracOwn 1) y) ⊢ ptstoSthL addrs.
+  Proof.
+    intros nd.
+    induction nd as [|a l anl ndl]; cbn.
+    - now iIntros "_".
+    - iIntros "Hmem".
+      rewrite big_sepM_insert.
+      iDestruct "Hmem" as "[Hmema Hmem]".
+      iSplitL "Hmema".
+      + now iExists (μ a).
+      + now iApply IHndl.
+      + apply not_elem_of_list_to_map_1.
+        change (fmap fst ?l) with (map fst l).
+        now rewrite map_map map_id.
+  Qed.
+
+  Lemma femtokernel_splitMemory `{sailGS Σ} {μ : Memory} :
+    mem_has_instrs μ 0 femtokernel_init ->
+    mem_has_instrs μ 72 femtokernel_handler ->
+    μ 84 = 42 ->
+    mem_res sailGS_memGS μ ⊢ |={⊤}=>
+      ptsto_instrs 0 femtokernel_init ∗
+      ptsto_instrs 72 femtokernel_handler ∗
+      interp_ptsto_readonly 84 42 ∗
+      ptstoSthL advAddrs.
+  Proof.
+    iIntros (Hinit Hhandler Hft) "Hmem".
+    unfold mem_res, initMemMap.
+    rewrite liveAddrs_split.
+    rewrite ?map_app ?list_to_map_app ?big_sepM_union.
+    - iDestruct "Hmem" as "(Hinit & Hhandler & Hfortytwo & _ & Hadv)".
+      iSplitL "Hinit".
+      now iApply (intro_ptsto_instrs (μ := μ)).
+      iSplitL "Hhandler".
+      now iApply (intro_ptsto_instrs (μ := μ)).
+      iSplitL "Hfortytwo".
+      rewrite big_sepM_singleton.
+      cbn.
+      unfold interp_ptsto_readonly.
+      change (gen_heap.mapsto 84 (dfrac.DfracOwn 1) (μ 84)) with (interp_ptsto 84 (μ 84)).
+      rewrite Hft.
+      iMod (inv.inv_alloc femto_inv_ns ⊤ (interp_ptsto 84 42) with "Hfortytwo") as "Hinv".
+      now iModIntro.
+
+      cbn.
+      iModIntro.
+      iApply (intro_ptstoSthL μ).
+      {apply NoDup_seqZ.}
+      done.
+      all: admit.
+  Admitted.
+
+  Lemma interp_ptsto_valid `{sailGS Σ} {μ a v} :
+    ⊢ mem_inv _ μ -∗ interp_ptsto a v -∗ ⌜μ a = v⌝.
+  Proof.
+    unfold interp_ptsto, mem_inv.
+    iIntros "(%memmap & Hinv & %link) Hptsto".
+    iDestruct (gen_heap.gen_heap_valid with "Hinv Hptsto") as "%x".
+    iPureIntro.
+    now apply (map_Forall_lookup_1 _ _ _ _ link).
+  Qed.
+
+  Lemma femtokernel_endToEnd {γ γ' : RegStore} {μ μ' : Memory}
+        {δ δ' : CStore [ctx]} {s' : Stm [ctx] ty.unit} :
+    mem_has_instrs μ 0 femtokernel_init ->
+    mem_has_instrs μ 72 femtokernel_handler ->
+    μ 84 = 42 ->
+    read_register γ cur_privilege = Machine ->
+    read_register γ pmp0cfg = femtokernel_default_pmpcfg ->
+    read_register γ pmp1cfg = femtokernel_default_pmpcfg ->
+    read_register γ pc = 0 ->
+    ⟨ γ, μ, δ, fun_loop ⟩ --->* ⟨ γ', μ', δ', s' ⟩ ->
+    μ' 84 = 42.
+  Proof.
+    intros μinit μhandler μft γcurpriv γpmp0cfg γpmp1cfg γpc steps.
+    refine (adequacy_gen (Q := fun _ _ _ _ => True%I) (μ' 84 = 42) steps _).
+    iIntros (Σ' H).
+    unfold own_regstore.
+    cbn.
+    iIntros "(Hmem & Hpc & Hnpc & Hmstatus & Hmtvec & Hmcause & Hmepc & Hcurpriv & Hx1 & Hx2 & Hx3 & Hx4 & Hx5 & Hx6 & Hx7 & Hpmp0cfg & Hpmp1cfg & Hpmpaddr0 & Hpmpaddr1 & _)".
+    rewrite γcurpriv γpmp0cfg γpmp1cfg γpc.
+    (* TODO: need to allocate an invariant here! *)
+    iMod (femtokernel_splitMemory with "Hmem") as "(Hinit & Hhandler & #Hfortytwo & Hadv)";
+      try assumption.
+    iModIntro.
+    iSplitR "".
+    - destruct (env.nilView δ).
+      iApply femtokernel_init_safe.
+      iFrame.
+      iSplitL "Hmstatus". { now iExists _. }
+      iSplitL "Hmtvec". { now iExists _. }
+      iSplitL "Hmcause". { now iExists _. }
+      iSplitL "Hmepc". { now iExists _. }
+      iSplitL "Hx1 Hx2 Hx3 Hx4 Hx5 Hx6 Hx7".
+      {rewrite Model.RiscvPmpModel2.gprs_equiv. cbn.
+       iSplitL "Hx1". {now iExists _.}
+       iSplitL "Hx2". {now iExists _.}
+       iSplitL "Hx3". {now iExists _.}
+       iSplitL "Hx4". {now iExists _.}
+       iSplitL "Hx5". {now iExists _.}
+       iSplitL "Hx6". {now iExists _.}
+       now iExists _.
+      }
+      iSplitL "Hpmpaddr0". { now iExists _. }
+      iSplitL "Hpmpaddr1". { now iExists _. }
+      iSplitL "". { now done. }
+      now iExists _.
+    - iIntros "Hmem".
+      unfold interp_ptsto_readonly.
+      iInv "Hfortytwo" as ">Hptsto" "_".
+      iDestruct (interp_ptsto_valid with "Hmem Hptsto") as "res".
+      iApply fupd_mask_intro; first set_solver.
+      now iIntros "_".
+  Qed.
+  Print Assumptions femtokernel_endToEnd.
